src/CCLHashExec.v
@@ -3,22 +3,16 @@ Require Import Hashmap.
 Require Import Automation.
 
 Theorem exec_hashmap_le : forall T (p: cprog T)
-                            G tid sigma_i sigma out,
-    exec G tid (sigma_i, sigma) p out ->
+                            G tid sigma out,
+    exec G tid sigma p out ->
     match out with
-    | Finished _ sigma' _ => hashmap_le (Sigma.hm sigma) (Sigma.hm sigma')
+    | Finished sigma' _ => hashmap_le (Sigma.hm sigma) (Sigma.hm sigma')
     | Error => True
     end.
 Proof.
   intros.
-  remember (sigma_i, sigma).
   generalize dependent sigma.
-  generalize dependent sigma_i.
-  induction H; intros;
-    match goal with
-    | [ H: (_,_) = (_,_) |- _ ] =>
-      inversion H; subst; clear H
-    end; auto;
+  induction 1; intros; auto;
       repeat match goal with
              | [ x := _ |- _ ] => subst x
              | [ |- hashmap_le (Sigma.hm _) (Sigma.hm _) ] =>
@@ -26,7 +20,7 @@ Proof.
                       | [ sigma: Sigma |- _ ] => destruct sigma
                       end; simpl in *; reflexivity
              end.
-  - destruct sigma0.
+  - destruct sigma.
     destruct p;
       repeat match goal with
              | [ H: context[match ?d with | _ => _ end] |- _ ] =>
